ulib/FStar.Tactics.Derived.fst
@@ -35,7 +35,9 @@ let run_tactic (t:unit -> Tac unit)
 let goals () : Tac (list goal) = goals_of (get ())
 let smt_goals () : Tac (list goal) = smt_goals_of (get ())
 
-let fail (#a:Type) (m:string) = raise #a (TacticFailure m)
+let fail (#a:Type) (m:string)
+  : TAC a (fun ps0 p -> p (Failed (TacticFailure m) ps0))
+  = raise #a (TacticFailure m)
 
 (** Return the current *goal*, not its type. (Ignores SMT goals) *)
 let _cur_goal () : Tac goal =
@@ -103,13 +105,14 @@ This does not immediately run the SMT: it just dumps the goal in the
 SMT bin. Note, if you dump a proof-relevant goal there, the engine will
 later raise an error. *)
 let smt () : Tac unit =
-    match goals (), smt_goals () with
-    | [], _ -> fail "smt: no active goals"
-    | g::gs, gs' ->
-        begin
-        set_goals gs;
-        set_smt_goals (g :: gs')
-        end
+  let gs = goals () in
+  match gs, smt_goals () with
+  | [], _ -> fail "smt: no active goals"
+  | g::gs, gs' ->
+      begin
+      set_goals gs;
+      set_smt_goals (g :: gs')
+      end
 
 let idtac () : Tac unit = ()
 
@@ -231,7 +234,8 @@ on the second, returning both results (and concatenating remaining goals). *)
 let divide (n:int) (l : unit -> Tac 'a) (r : unit -> Tac 'b) : Tac ('a * 'b) =
     if n < 0 then
       fail "divide: negative n";
-    let gs, sgs = goals (), smt_goals () in
+    let gs = goals () in
+    let sgs = smt_goals () in
     let gs1, gs2 = List.Tot.Base.splitAt n gs in
 
     set_goals gs1; set_smt_goals [];
@@ -263,7 +267,9 @@ let focus (t : unit -> Tac 'a) : Tac 'a =
         x
 
 (** Similar to [dump], but only dumping the current goal. *)
-let dump1 (m : string) = focus (fun () -> dump m)
+let dump1 (m : string)
+  : Tac unit
+  = focus (fun () -> dump m)
 
 let rec mapAll (t : unit -> Tac 'a) : Tac (list 'a) =
     match goals () with
@@ -277,7 +283,8 @@ let rec iterAll (t : unit -> Tac unit) : Tac unit =
     | _::_ -> let _ = divide 1 t (fun () -> iterAll t) in ()
 
 let iterAllSMT (t : unit -> Tac unit) : Tac unit =
-    let gs, sgs = goals (), smt_goals () in
+  let gs = goals () in
+  let sgs = smt_goals () in
     set_goals sgs;
     set_smt_goals [];
     iterAll t;
@@ -337,7 +344,7 @@ let guard (b : bool) : TacH unit (requires (fun _ -> True))
     else ()
 
 let try_with (f : unit -> Tac 'a) (h : exn -> Tac 'a) : Tac 'a =
-    match catch f with
+    match catch #'a f with
     | Inl e -> h e
     | Inr x -> x
 
@@ -359,7 +366,7 @@ let first (ts : list (unit -> Tac 'a)) : Tac 'a =
     L.fold_right (<|>) ts (fun () -> fail "no tactics to try") ()
 
 let rec repeat (#a:Type) (t : unit -> Tac a) : Tac (list a) =
-    match catch t with
+    match catch #a t with
     | Inl _ -> []
     | Inr x -> x :: repeat t
 
@@ -380,8 +387,9 @@ let norm_term (s : list norm_step) (t : term) : Tac term =
 expected to be similar, and therefore easier to prove at once by the SMT
 solver. TODO: would be nice to try to join them in a more meaningful
 way, as the order can matter. *)
-let join_all_smt_goals () =
-  let gs, sgs = goals (), smt_goals () in
+let join_all_smt_goals () : Tac unit =
+  let gs = goals () in
+  let sgs = smt_goals () in
   set_smt_goals [];
   set_goals sgs;
   repeat' join;
@@ -396,7 +404,9 @@ let discard (tau : unit -> Tac 'a) : unit -> Tac unit =
 let rec repeatseq (#a:Type) (t : unit -> Tac a) : Tac unit =
     let _ = trytac (fun () -> (discard t) `seq` (discard (fun () -> repeatseq t))) in ()
 
-let tadmit () = tadmit_t (`())
+let tadmit ()
+  : Tac unit
+  = tadmit_t (`())
 
 let admit1 () : Tac unit =
     tadmit ()
@@ -543,7 +553,7 @@ let l_to_r (lems:list term) : Tac unit =
     let first_or_trefl () : Tac unit =
         fold_left (fun k l () ->
                     (fun () -> apply_lemma l)
-                    `or_else` k)
+                    `or_else` k <: Tac unit)
                   trefl lems () in
     pointwise first_or_trefl
 
@@ -568,13 +578,13 @@ let grewrite_eq (b:binder) : Tac unit =
   match term_as_formula (type_of_binder b) with
   | Comp (Eq _) l r ->
     grewrite l r;
-    iseq [idtac; (fun () -> exact (binder_to_term b))]
+    iseq [idtac; (fun () -> exact (binder_to_term b) <: Tac unit)]
   | _ ->
     begin match term_as_formula' (type_of_binder b) with
     | Comp (Eq _) l r ->
       grewrite l r;
-      iseq [idtac; (fun () -> apply_lemma (`__un_sq_eq);
-                              exact (binder_to_term b))]
+      iseq [idtac; (fun () -> (apply_lemma (`__un_sq_eq);
+                              exact (binder_to_term b)) <: Tac unit)]
     | _ ->
       fail "grewrite_eq: binder type is not an equality"
     end
@@ -728,13 +738,13 @@ let add_elem (t : unit -> Tac 'a) : Tac 'a = focus (fun () ->
 let specialize (#a:Type) (f:a) (l:list string) :unit -> Tac unit
   = fun () -> solve_then (fun () -> exact (quote f)) (fun () -> norm [delta_only l; iota; zeta])
 
-let tlabel (l:string) =
+let tlabel (l:string) : Tac unit =
     match goals () with
     | [] -> fail "tlabel: no goals"
     | h::t ->
         set_goals (set_label l h :: t)
 
-let tlabel' (l:string) =
+let tlabel' (l:string) : Tac unit =
     match goals () with
     | [] -> fail "tlabel': no goals"
     | h::t ->
@@ -856,7 +866,7 @@ and visit_comp (ff : term -> Tac term) (c : comp) : Tac comp =
 
     | C_Eff us eff res args ->
         let res = visit_tm ff res in
-        let args = map (fun (a, q) -> (visit_tm ff a, q)) args in
+        let args = map (fun (a, q) -> (visit_tm ff a, q) <: Tac (term * aqualv)) args in
         C_Eff us eff res args
   in
   pack_comp cv'
