ulib/FStar.Tactics.SyntaxHelpers.fst
@@ -45,7 +45,9 @@ let collect_abs t =
 
 (* Copied from FStar.Tactics.Derived *)
 private
-let fail (#a:Type) (m:string) = raise #a (TacticFailure m)
+let fail (#a:Type) (m:string)
+  : TAC a (fun ps0 p -> p (Failed (TacticFailure m) ps0))
+  = raise #a (TacticFailure m)
 
 let rec mk_arr (bs: list binder) (cod : comp) : Tac term =
     match bs with
